---
title: Ableitungen
---
$$
f(x) = e^x \Rightarrow f'(x) = e^x
$$
$$
f(x) = e^{ax} \Rightarrow f'(x) = a*e^{ax}
$$ (Kettenregel)
$$
f(x) = ln(x) \Rightarrow f'(x) = \frac{1}{x}
$$
$$
f(x) = ln(a * x) \Rightarrow f'(x) = \frac{1}{a * x} * a = \frac{1}{x}
$$
$$
f(x) = ln(a * x + b) \Rightarrow f'(x) = \frac{a}{a * x + b}
$$
$$
f(x) = a * ln(x) + b \Rightarrow f'(x) = \frac{a}{x}
$$
$$
f(x) = a * ln(x) + b \Rightarrow f'(x) = \frac{a}{x}
$$
$$
f(x) = 1 - e^{-ax} \Rightarrow f'(x) = -e^{-ax} * (-a) = a*e^{-ax}
$$ (Kettenregel)
